
\begin{figure}
	\centering
	\fixedCodeFrame{
	\small
        ~\\[2mm]

        \fbox{$E\vdash c :: k$}
          \begin{equation}
              \infer{E\vdash \alpha :: E(\alpha)}
              {\strut}
              \label{eq:f-k-var}
          \end{equation}

          \begin{equation}
              \infer{E \vdash \inj(\tau^n) :: \Omega_1 \to \ldots \Omega_n \to \Omega}
              {\strut}
              \label{eq:f-k-at}
          \end{equation}

          \begin{equation}
              \infer{E \vdash \newx(n) :: \Omega_1 \to \ldots \Omega_n
                \to \Omega}
              {\strut}
              \label{eq:f-k-new}
          \end{equation}

          \begin{equation}
              \infer{E \vdash (\lambda\alpha::k.c) :: k \to k'}
              {E[\alpha::k]\vdash c :: k'}
              \label{eq:f-k-lam}
          \end{equation}

          \begin{equation}
              \infer{E \vdash c_1(c_2) :: k_2}
              {E\vdash c_1 :: k_1 \to k_2\qquad E\vdash c_2 :: k_1}
              \label{eq:f-k-app}
           \end{equation}

           \begin{equation}
             \infer{E \vdash \{l_1=c_1,\ldots,l_n=c_n\} 
               :: \{l_1::k_1,\ldots,l_n::k_n\}}
             {E\vdash c_1::k_1\ldots E\vdash c_n::k_n}
             \label{eq:f-k-rec}
           \end{equation}

           \begin{equation}
             \infer{E\vdash c.l :: k}
             {E\vdash c :: \{lks\}\qquad l::k\in\{lks\}}
             \label{eq:f-k-proj}
           \end{equation}
            
        }
        \caption{F$_\omega$ well-kinding}
        \label{fig:fomega-kinding}
\end{figure}
